DynamoDbEncryption/dafny/StructuredEncryption/src/AwsCryptographyDbEncryptionSdkStructuredEncryptionOperations.dfy
@@ -54,22 +54,22 @@ module AwsCryptographyDbEncryptionSdkStructuredEncryptionOperations refines Abst
   predicate EncryptStructureEnsuresPublicly(
     input: EncryptStructureInput,
     output: Result<EncryptStructureOutput, Error>) {
-      // Input and output types must be the same, and this constraint is useful to Dafny users
+    // Input and output types must be the same, and this constraint is useful to Dafny users
     && (output.Success? && input.plaintextStructure.content.DataMap? ==> output.value.encryptedStructure.content.DataMap?)
     && (output.Success? && input.plaintextStructure.content.DataList? ==> output.value.encryptedStructure.content.DataList?)
     && (output.Success? && input.plaintextStructure.content.Terminal? ==> output.value.encryptedStructure.content.Terminal?)
-    // Ensure the CryptoSchema in the ParsedHeader matches the input crypto Schema, minus any DO_NOTHING terminals
+       // Ensure the CryptoSchema in the ParsedHeader matches the input crypto Schema, minus any DO_NOTHING terminals
     && (output.Success? ==>
-      // For now we only support encrypting flat maps
-      && output.value.parsedHeader.cryptoSchema.content.SchemaMap?
-      && var headerSchema := output.value.parsedHeader.cryptoSchema.content.SchemaMap;
-      && CryptoSchemaMapIsFlat(headerSchema)
-      && input.cryptoSchema.content.SchemaMap?
-      && var inputSchema := input.cryptoSchema.content.SchemaMap;
-      && CryptoSchemaMapIsFlat(inputSchema)
-      && (forall k :: k in headerSchema ==> k in inputSchema && inputSchema[k] == headerSchema[k])
-      && (forall v :: v in headerSchema.Values ==> IsAuthAttr(v.content.Action))
-    )
+          // For now we only support encrypting flat maps
+          && output.value.parsedHeader.cryptoSchema.content.SchemaMap?
+          && var headerSchema := output.value.parsedHeader.cryptoSchema.content.SchemaMap;
+          && CryptoSchemaMapIsFlat(headerSchema)
+          && input.cryptoSchema.content.SchemaMap?
+          && var inputSchema := input.cryptoSchema.content.SchemaMap;
+          && CryptoSchemaMapIsFlat(inputSchema)
+          && (forall k :: k in headerSchema ==> k in inputSchema && inputSchema[k] == headerSchema[k])
+          && (forall v :: v in headerSchema.Values ==> IsAuthAttr(v.content.Action))
+       )
   }
 
   // given a list of fields, return only those that should be encrypted, according to the legend
@@ -153,43 +153,43 @@ module AwsCryptographyDbEncryptionSdkStructuredEncryptionOperations refines Abst
   )
     returns (ret : Result<CMP.EncryptionMaterials, Error>)
     ensures ret.Success? ==>
-      && var mat := ret.value;
-      && Materials.EncryptionMaterialsHasPlaintextDataKey(mat)
-      && ValidSuite(mat.algorithmSuite)
+              && var mat := ret.value;
+              && Materials.EncryptionMaterialsHasPlaintextDataKey(mat)
+              && ValidSuite(mat.algorithmSuite)
 
-      //= specification/structured-encryption/encrypt-structure.md#retrieve-encryption-materials
-      //= type=implication
-      //# This operation MUST obtain a set of encryption materials by calling
-      //# [Get Encryption Materials](../../submodules/MaterialProviders/aws-encryption-sdk-specification/framework/cmm-interface.md#get-encryption-materials)
-      //# on the input [CMM](#cmm).
-      && (|cmm.History.GetEncryptionMaterials| == |old(cmm.History.GetEncryptionMaterials)| + 1)
-      && Seq.Last(cmm.History.GetEncryptionMaterials).output.Success?
-      && var getEncIn := Seq.Last(cmm.History.GetEncryptionMaterials).input;
-      //= specification/structured-encryption/encrypt-structure.md#retrieve-encryption-materials
-      //= type=implication
-      //# - Encryption Context: If provided, this MUST be the [input encryption context](#encryption-context);
-      //# otherwise, this is an empty encryption context.
-      && (|| (encryptionContext.None? && getEncIn.encryptionContext == map[])
-          || (encryptionContext.Some? && getEncIn.encryptionContext == encryptionContext.value))
+              //= specification/structured-encryption/encrypt-structure.md#retrieve-encryption-materials
+              //= type=implication
+              //# This operation MUST obtain a set of encryption materials by calling
+              //# [Get Encryption Materials](../../submodules/MaterialProviders/aws-encryption-sdk-specification/framework/cmm-interface.md#get-encryption-materials)
+              //# on the input [CMM](#cmm).
+              && (|cmm.History.GetEncryptionMaterials| == |old(cmm.History.GetEncryptionMaterials)| + 1)
+              && Seq.Last(cmm.History.GetEncryptionMaterials).output.Success?
+              && var getEncIn := Seq.Last(cmm.History.GetEncryptionMaterials).input;
+              //= specification/structured-encryption/encrypt-structure.md#retrieve-encryption-materials
+              //= type=implication
+              //# - Encryption Context: If provided, this MUST be the [input encryption context](#encryption-context);
+              //# otherwise, this is an empty encryption context.
+              && (|| (encryptionContext.None? && getEncIn.encryptionContext == map[])
+                  || (encryptionContext.Some? && getEncIn.encryptionContext == encryptionContext.value))
 
-      //= specification/structured-encryption/encrypt-structure.md#retrieve-encryption-materials
-      //= type=implication
-      //# - Commitment Policy: This MUST be
-      //# [REQUIRE_ENCRYPT_REQUIRE_DECRYPT](../../submodules/MaterialProviders/aws-encryption-sdk-specification/framework/commitment-policy.md#esdkrequire_encrypt_require_decrypt).
-      && getEncIn.commitmentPolicy == DBE_COMMITMENT_POLICY
+              //= specification/structured-encryption/encrypt-structure.md#retrieve-encryption-materials
+              //= type=implication
+              //# - Commitment Policy: This MUST be
+              //# [REQUIRE_ENCRYPT_REQUIRE_DECRYPT](../../submodules/MaterialProviders/aws-encryption-sdk-specification/framework/commitment-policy.md#esdkrequire_encrypt_require_decrypt).
+              && getEncIn.commitmentPolicy == DBE_COMMITMENT_POLICY
 
-      //= specification/structured-encryption/encrypt-structure.md#retrieve-encryption-materials
-      //= type=implication
-      //# - Max Plaintext Length: This field MUST be the result of the calculation `encryptedTerminalDataNum * 2 + totalEncryptedTerminalValuesSize`
-      // - `encryptedTerminalDataNum` is the number of [Terminal Data](./structures.md#terminal-data)
-      //   in the [input Structured Data](#structured-data) being encrypted,
-      //   as defined by the [input Crypto Schema](#crypto-schema).
-      // - `totalEncryptedTerminalValuesSize` is the sum of the length of all [Terminal Values](./structures.md#terminal-value)
-      //   in the [input Structured Data](#structured-data) being encrypted,
-      //   as defined by the [input Crypto Schema](#crypto-schema).
-      && var maxLength :=  encryptedTerminalDataNum * 2 + totalEncryptedTerminalValuesSize;
-      && maxLength < INT64_MAX_LIMIT
-      && (getEncIn.maxPlaintextLength == Some(maxLength as int64))
+              //= specification/structured-encryption/encrypt-structure.md#retrieve-encryption-materials
+              //= type=implication
+              //# - Max Plaintext Length: This field MUST be the result of the calculation `encryptedTerminalDataNum * 2 + totalEncryptedTerminalValuesSize`
+              // - `encryptedTerminalDataNum` is the number of [Terminal Data](./structures.md#terminal-data)
+              //   in the [input Structured Data](#structured-data) being encrypted,
+              //   as defined by the [input Crypto Schema](#crypto-schema).
+              // - `totalEncryptedTerminalValuesSize` is the sum of the length of all [Terminal Values](./structures.md#terminal-value)
+              //   in the [input Structured Data](#structured-data) being encrypted,
+              //   as defined by the [input Crypto Schema](#crypto-schema).
+              && var maxLength :=  encryptedTerminalDataNum * 2 + totalEncryptedTerminalValuesSize;
+              && maxLength < INT64_MAX_LIMIT
+              && (getEncIn.maxPlaintextLength == Some(maxLength as int64))
 
     modifies cmm.Modifies
     requires cmm.ValidState()
@@ -224,7 +224,7 @@ module AwsCryptographyDbEncryptionSdkStructuredEncryptionOperations refines Abst
   }
 
   type EncryptCanon = c: EncryptCanonData | ValidEncryptCanon?(c)
-  witness *
+    witness *
 
   // for Encrypt, the data necessary to construct the Intermediate Encrypted Structured Data
   datatype EncryptCanonData = EncryptCanonData (
@@ -250,7 +250,7 @@ module AwsCryptographyDbEncryptionSdkStructuredEncryptionOperations refines Abst
   }
 
   type DecryptCanon = c: DecryptCanonData | ValidDecryptCanon?(c)
-  witness *
+    witness *
 
   // for Decrypt, the data necessary to construct the Intermediate Encrypted Structured Data
   datatype DecryptCanonData = DecryptCanonData (
@@ -309,30 +309,30 @@ module AwsCryptographyDbEncryptionSdkStructuredEncryptionOperations refines Abst
     : (ret : Result<EncryptCanon, Error>)
     requires schema.Keys == data.Keys
     ensures ret.Success? ==>
-      && var r := ret.value;
-      
-      //= specification/structured-encryption/encrypt-structure.md#calculate-intermediate-encrypted-structured-data
-      //= type=implication
-      //# For every [input Terminal Data](./structures.md#terminal-data)
-      //# in the [input Structured Data](#structured-data),
-      //# a Terminal Data MUST exist with the same [canonical path](./header.md#canonical-path)
-      //# in Intermediate Encrypted Structured Data,
-      //# if the [Crypto Schema](#crypto-schema)
-      //# indicates a [Crypto Action](./structures.md#crypto-action)
-      //# other than [DO_NOTHING](./structures.md#DO_NOTHING).
-      && (forall k <- data :: schema[k].content.Action == DO_NOTHING || Paths.SimpleCanon(tableName, k) in ret.value.data_c)
+              && var r := ret.value;
 
-      //= specification/structured-encryption/encrypt-structure.md#calculate-intermediate-encrypted-structured-data
-      //= type=implication
-      //# For every [Terminal Data](./structures.md#terminal-data)
-      //# in the Intermediate Encrypted Structured Data
-      //# a Terminal Data MUST exist with the same [canonical path](./header.md#canonical-path)
-      //# in the [input Structured Data](#structured-data).
-      && (forall k <- ret.value.data_c :: (exists x :: x in data && k == Paths.SimpleCanon(tableName, x)))
+              //= specification/structured-encryption/encrypt-structure.md#calculate-intermediate-encrypted-structured-data
+              //= type=implication
+              //# For every [input Terminal Data](./structures.md#terminal-data)
+              //# in the [input Structured Data](#structured-data),
+              //# a Terminal Data MUST exist with the same [canonical path](./header.md#canonical-path)
+              //# in Intermediate Encrypted Structured Data,
+              //# if the [Crypto Schema](#crypto-schema)
+              //# indicates a [Crypto Action](./structures.md#crypto-action)
+              //# other than [DO_NOTHING](./structures.md#DO_NOTHING).
+              && (forall k <- data :: schema[k].content.Action == DO_NOTHING || Paths.SimpleCanon(tableName, k) in ret.value.data_c)
 
-      && ret.value.cryptoSchema.content.SchemaMap?
-      && var trimmedSchema := ret.value.cryptoSchema.content.SchemaMap;
-      && (forall k :: k in trimmedSchema ==> k in schema && trimmedSchema[k] == schema[k])
+              //= specification/structured-encryption/encrypt-structure.md#calculate-intermediate-encrypted-structured-data
+              //= type=implication
+              //# For every [Terminal Data](./structures.md#terminal-data)
+              //# in the Intermediate Encrypted Structured Data
+              //# a Terminal Data MUST exist with the same [canonical path](./header.md#canonical-path)
+              //# in the [input Structured Data](#structured-data).
+              && (forall k <- ret.value.data_c :: (exists x :: x in data && k == Paths.SimpleCanon(tableName, x)))
+
+              && ret.value.cryptoSchema.content.SchemaMap?
+              && var trimmedSchema := ret.value.cryptoSchema.content.SchemaMap;
+              && (forall k :: k in trimmedSchema ==> k in schema && trimmedSchema[k] == schema[k])
   {
     var fieldMap := GetFieldMap(tableName, data, schema);
 
@@ -375,16 +375,16 @@ module AwsCryptographyDbEncryptionSdkStructuredEncryptionOperations refines Abst
   ) : (ret : Result<DecryptCanon, Error>)
     requires authSchema.Keys == data.Keys
     ensures ret.Success? ==>
-      && |ret.value.signedFields_c| == |legend|
+              && |ret.value.signedFields_c| == |legend|
     ensures ret.Success? ==>
-      && (forall k :: k in data.Keys && authSchema[k].content.Action.SIGN? ==> Paths.SimpleCanon(tableName, k) in ret.value.data_c.Keys)
+              && (forall k :: k in data.Keys && authSchema[k].content.Action.SIGN? ==> Paths.SimpleCanon(tableName, k) in ret.value.data_c.Keys)
     ensures ret.Success? ==>
-      && (forall v :: v in ret.value.data_c.Values ==> v in data.Values)
+              && (forall v :: v in ret.value.data_c.Values ==> v in data.Values)
     ensures ret.Success? ==>
-      && ret.value.cryptoSchema.content.SchemaMap?
-      && CryptoSchemaMapIsFlat(ret.value.cryptoSchema.content.SchemaMap)
-      && AuthSchemaIsFlat(authSchema)
-      && ValidParsedCryptoSchema(ret.value.cryptoSchema.content.SchemaMap, authSchema, tableName)
+              && ret.value.cryptoSchema.content.SchemaMap?
+              && CryptoSchemaMapIsFlat(ret.value.cryptoSchema.content.SchemaMap)
+              && AuthSchemaIsFlat(authSchema)
+              && ValidParsedCryptoSchema(ret.value.cryptoSchema.content.SchemaMap, authSchema, tableName)
     ensures ret.Success? ==> forall k <- ret.value.contextFields :: k in data
   {
     //= specification/structured-encryption/decrypt-structure.md#calculate-signed-and-encrypted-field-lists
@@ -397,65 +397,65 @@ module AwsCryptographyDbEncryptionSdkStructuredEncryptionOperations refines Abst
     reveal Maps.Injective();
     Paths.SimpleCanonUnique(tableName);
     var fieldMap := map k <- data | authSchema[k].content.Action == SIGN ::
-      Paths.SimpleCanon(tableName, k) := k;
+                      Paths.SimpleCanon(tableName, k) := k;
     assert Maps.Injective(fieldMap);
     assert forall k <- fieldMap :: fieldMap[k] in data;
-  
+
     var data_c := map k <- fieldMap :: k := data[fieldMap[k]];
     var signedFields_c := SortedSets.ComputeSetToOrderedSequence2(data_c.Keys, ByteLess);
 
     if |legend| < |signedFields_c| then
       Failure(E("Schema changed : something that was unsigned is now signed."))
-    else 
+    else
     if |legend| > |signedFields_c| then
       Failure(E("Schema changed : something that was signed is now unsigned."))
     else
 
-    //= specification/structured-encryption/decrypt-structure.md#calculate-signed-and-encrypted-field-lists
-    //# The `encrypted field list` MUST be all fields in the `signed field list`
-    //# for which the corresponding byte in the [Encrypt Legend](header.md.#encrypt-legend)
-    //# is `0x65` indicating [Encrypt and Sign](header.md.#encrypt-legend-bytes),
-    //# sorted by the field's [canonical path](./header.md#canonical-path).
-    var encFields_c : seq<CanonicalPath> := FilterEncrypted(signedFields_c, legend);
-    :- Need(|encFields_c| < (UINT32_LIMIT / 3), E("Too many encrypted fields."));
+      //= specification/structured-encryption/decrypt-structure.md#calculate-signed-and-encrypted-field-lists
+      //# The `encrypted field list` MUST be all fields in the `signed field list`
+      //# for which the corresponding byte in the [Encrypt Legend](header.md.#encrypt-legend)
+      //# is `0x65` indicating [Encrypt and Sign](header.md.#encrypt-legend-bytes),
+      //# sorted by the field's [canonical path](./header.md#canonical-path).
+      var encFields_c : seq<CanonicalPath> := FilterEncrypted(signedFields_c, legend);
+      :- Need(|encFields_c| < (UINT32_LIMIT / 3), E("Too many encrypted fields."));
 
-    var contextFields : seq<string> := FilterContext(fieldMap, signedFields_c, legend, data);
-    assert forall k <- contextFields :: k in data;
+      var contextFields : seq<string> := FilterContext(fieldMap, signedFields_c, legend, data);
+      assert forall k <- contextFields :: k in data;
 
-    var actionMap := map k <- fieldMap ::
-      fieldMap[k] := if Paths.SimpleCanon(tableName, fieldMap[k]) in encFields_c then
-        CryptoSchema(
-          content := CryptoSchemaContent.Action(ENCRYPT_AND_SIGN),
-          attributes := None
-        )
-      else
-        CryptoSchema(
-          content := CryptoSchemaContent.Action(SIGN_ONLY),
-          attributes := None
-        );
-    var cryptoSchema := CryptoSchema(
-      content := CryptoSchemaContent.SchemaMap(actionMap),
-      attributes := None
-    );
+      var actionMap := map k <- fieldMap ::
+                         fieldMap[k] := if Paths.SimpleCanon(tableName, fieldMap[k]) in encFields_c then
+                                          CryptoSchema(
+                                            content := CryptoSchemaContent.Action(ENCRYPT_AND_SIGN),
+                                            attributes := None
+                                          )
+                                        else
+                                          CryptoSchema(
+                                            content := CryptoSchemaContent.Action(SIGN_ONLY),
+                                            attributes := None
+                                          );
+      var cryptoSchema := CryptoSchema(
+                            content := CryptoSchemaContent.SchemaMap(actionMap),
+                            attributes := None
+                          );
 
-    var c := DecryptCanonData(
-      encFields_c,
-      signedFields_c,
-      data_c,
-      cryptoSchema,
-      contextFields
-    );
+      var c := DecryptCanonData(
+                 encFields_c,
+                 signedFields_c,
+                 data_c,
+                 cryptoSchema,
+                 contextFields
+               );
 
-    assert |data_c| == |actionMap| by {
-      assert data_c.Keys == fieldMap.Keys;
-      assert actionMap.Keys == fieldMap.Values;
-      LemmaInjectiveImpliesUniqueValues(fieldMap);
-    }
+      assert |data_c| == |actionMap| by {
+        assert data_c.Keys == fieldMap.Keys;
+        assert actionMap.Keys == fieldMap.Values;
+        LemmaInjectiveImpliesUniqueValues(fieldMap);
+      }
 
-    assert exists tableName ::
-      (forall k :: k in c.cryptoSchema.content.SchemaMap ==> Paths.SimpleCanon(tableName, k) in c.data_c);
+      assert exists tableName ::
+          (forall k :: k in c.cryptoSchema.content.SchemaMap ==> Paths.SimpleCanon(tableName, k) in c.data_c);
 
-    Success(c)
+      Success(c)
   }
 
   method GetV2EncryptionContext(schema : FlatSchemaMap, oldContext : CMP.EncryptionContext, record : FlatDataMap)
@@ -474,11 +474,11 @@ module AwsCryptographyDbEncryptionSdkStructuredEncryptionOperations refines Abst
     var newContext := oldContext;
     for i := 0 to |fields| {
       var fieldStr := fields[i];
-      var fieldUtf8 :- UTF8.Encode(fieldStr).MapFailure(e => E(e));
-      var attr := record[fieldStr].content.Terminal;
-      :- Need(attr.typeId == STRING || attr.typeId == NUMBER, E(""));
-      :- Need(ValidUTF8Seq(attr.value), E("Internal error. Value for " + fieldStr + " was not utf8."));
-      newContext := oldContext[fieldUtf8 := attr.value];
+      var newFieldStr := SE_ATTR_PREFIX + fieldStr;
+      var fieldUtf8 : ValidUTF8Bytes :- UTF8.Encode(newFieldStr).MapFailure(e => E(e));
+      var attr : StructuredDataTerminal := record[fieldStr].content.Terminal;
+      var attrStr : ValidUTF8Bytes := EncodeTerminal(attr);
+      newContext := oldContext[fieldUtf8 := attrStr];
     }
     return Success(newContext);
   }
@@ -486,48 +486,48 @@ module AwsCryptographyDbEncryptionSdkStructuredEncryptionOperations refines Abst
   method {:vcs_split_on_every_assert} EncryptStructure(config: InternalConfig, input: EncryptStructureInput)
     returns (output: Result<EncryptStructureOutput, Error>)
     ensures output.Success? ==>
-      //= specification/structured-encryption/encrypt-structure.md#structured-data
-      //= type=implication
-      //# This Structured Data MUST be a [Structured Data Map](./structures.md#structured-data-map).
-      && input.plaintextStructure.content.DataMap?
+              //= specification/structured-encryption/encrypt-structure.md#structured-data
+              //= type=implication
+              //# This Structured Data MUST be a [Structured Data Map](./structures.md#structured-data-map).
+              && input.plaintextStructure.content.DataMap?
 
-      //= specification/structured-encryption/encrypt-structure.md#structured-data
-      //= type=implication
-      //# This Structured Data MUST NOT already contain data located at the [header index](./header.md#header-index)
-      //# or the [footer index](./footer.md#footer-index).
-      && var plainRecord := input.plaintextStructure.content.DataMap;
-      && DataMapIsFlat(plainRecord)
-      && HeaderField !in plainRecord
-      && FooterField !in plainRecord
+              //= specification/structured-encryption/encrypt-structure.md#structured-data
+              //= type=implication
+              //# This Structured Data MUST NOT already contain data located at the [header index](./header.md#header-index)
+              //# or the [footer index](./footer.md#footer-index).
+              && var plainRecord := input.plaintextStructure.content.DataMap;
+              && DataMapIsFlat(plainRecord)
+              && HeaderField !in plainRecord
+              && FooterField !in plainRecord
 
-      //= specification/structured-encryption/encrypt-structure.md#crypto-schema
-      //= type=implication
-      //# The Crypto Schema MUST explicitly configure a [Crypto Action](./structures.md#crypto-action) for every
-      //# [Terminal Data](./structures.md#terminal-data) that exists on the [input Structured Data](#structured-data),
-      //# and MUST NOT describe Crypto Actions for locations within the input Structured Data that either
-      //# do not exist, or contain non-Terminal Data structures;
-      //# otherwise, this operation operation MUST yield an error.
-      && input.cryptoSchema.content.SchemaMap?
-      && var cryptoSchema := input.cryptoSchema.content.SchemaMap;
-      && CryptoSchemaMapIsFlat(cryptoSchema)
-      && plainRecord.Keys == cryptoSchema.Keys
+              //= specification/structured-encryption/encrypt-structure.md#crypto-schema
+              //= type=implication
+              //# The Crypto Schema MUST explicitly configure a [Crypto Action](./structures.md#crypto-action) for every
+              //# [Terminal Data](./structures.md#terminal-data) that exists on the [input Structured Data](#structured-data),
+              //# and MUST NOT describe Crypto Actions for locations within the input Structured Data that either
+              //# do not exist, or contain non-Terminal Data structures;
+              //# otherwise, this operation operation MUST yield an error.
+              && input.cryptoSchema.content.SchemaMap?
+              && var cryptoSchema := input.cryptoSchema.content.SchemaMap;
+              && CryptoSchemaMapIsFlat(cryptoSchema)
+              && plainRecord.Keys == cryptoSchema.Keys
 
-      //= specification/structured-encryption/encrypt-structure.md#crypto-schema
-      //= type=implication
-      //# The Crypto Schema MUST include at least one [ENCRYPT_AND_SIGN Crypto Action](./structures.md#encryptandsign) or
-      //# [SIGN_ONLY Crypto Action](./structures.md#signonly);
-      //# otherwise, this operation MUST yield an error.
-      && (exists k <- cryptoSchema :: cryptoSchema[k].content.Action != DO_NOTHING)
+              //= specification/structured-encryption/encrypt-structure.md#crypto-schema
+              //= type=implication
+              //# The Crypto Schema MUST include at least one [ENCRYPT_AND_SIGN Crypto Action](./structures.md#encryptandsign) or
+              //# [SIGN_ONLY Crypto Action](./structures.md#signonly);
+              //# otherwise, this operation MUST yield an error.
+              && (exists k <- cryptoSchema :: cryptoSchema[k].content.Action != DO_NOTHING)
 
-      //= specification/structured-encryption/encrypt-structure.md#encrypted-structured-data-1
-      //= type=implication
-      //# - The [Header Field](#header-field) MUST exist in the Encrypted Structured Data
-      && HeaderField in output.value.encryptedStructure.content.DataMap
+              //= specification/structured-encryption/encrypt-structure.md#encrypted-structured-data-1
+              //= type=implication
+              //# - The [Header Field](#header-field) MUST exist in the Encrypted Structured Data
+              && HeaderField in output.value.encryptedStructure.content.DataMap
 
-      //= specification/structured-encryption/encrypt-structure.md#encrypted-structured-data-1
-      //= type=implication
-      //# - The [Footer Field](#footer-field) MUST exist in the Encrypted Structured Data
-      && FooterField in output.value.encryptedStructure.content.DataMap
+              //= specification/structured-encryption/encrypt-structure.md#encrypted-structured-data-1
+              //= type=implication
+              //# - The [Footer Field](#footer-field) MUST exist in the Encrypted Structured Data
+              && FooterField in output.value.encryptedStructure.content.DataMap
 
   {
     :- Need(input.plaintextStructure.content.DataMap?, E("Input structure must be a DataMap"));
@@ -541,7 +541,7 @@ module AwsCryptographyDbEncryptionSdkStructuredEncryptionOperations refines Abst
     :- Need(CryptoSchemaMapIsFlat(cryptoSchema), E("Schema must be flat."));
     :- Need(forall k <- cryptoSchema :: ValidString(k), E("Schema has bad field name."));
     :- Need(exists k <- cryptoSchema :: IsAuthAttr(cryptoSchema[k].content.Action),
-      E("At least one field in the Crypto Schema must be ENCRYPT_AND_SIGN, CONTEXT_AND_SIGN or SIGN_ONLY."));
+            E("At least one field in the Crypto Schema must be ENCRYPT_AND_SIGN, CONTEXT_AND_SIGN or SIGN_ONLY."));
 
     :- Need(DataMapIsFlat(input.plaintextStructure.content.DataMap), E("Input DataMap must be flat."));
     var plainRecord : FlatDataMap := input.plaintextStructure.content.DataMap;
@@ -555,11 +555,11 @@ module AwsCryptographyDbEncryptionSdkStructuredEncryptionOperations refines Abst
     var encryptionContext := input.encryptionContext.UnwrapOr(map[]);
     encryptionContext :- GetV2EncryptionContext(cryptoSchema, encryptionContext, plainRecord);
     var mat :- GetStructuredEncryptionMaterials(
-                input.cmm,
-                Some(encryptionContext),
-                input.algorithmSuiteId,
-                |canonData.encFields_c|,
-                SumValueSize(canonData.encFields_c, canonData.data_c));
+      input.cmm,
+      Some(encryptionContext),
+      input.algorithmSuiteId,
+      |canonData.encFields_c|,
+      SumValueSize(canonData.encFields_c, canonData.data_c));
 
     var key : Key := mat.plaintextDataKey.value;
     var alg := mat.algorithmSuite;
@@ -591,11 +591,11 @@ module AwsCryptographyDbEncryptionSdkStructuredEncryptionOperations refines Abst
     var encryptedItems :- Crypt.Encrypt(config.primitives, alg, key, head, canonData.encFields_c, canonData.data_c);
 
     var result : map<string, StructuredData> := map k <- plainRecord | true :: k :=
-      var c := Paths.SimpleCanon(input.tableName, k);
-      if c in encryptedItems then
-        encryptedItems[c]
-      else
-        plainRecord[k];
+                                                                            var c := Paths.SimpleCanon(input.tableName, k);
+                                                                            if c in encryptedItems then
+                                                                              encryptedItems[c]
+                                                                            else
+                                                                              plainRecord[k];
 
     //= specification/structured-encryption/encrypt-structure.md#encrypted-structured-data-1
     //= type=implication
@@ -623,7 +623,7 @@ module AwsCryptographyDbEncryptionSdkStructuredEncryptionOperations refines Abst
     assert {:split_here} true;
 
     var footer :- Footer.CreateFooter(config.primitives, mat, canonData.signedFields_c,
-                canonData.encFields_c, encryptedItems, canonData.data_c, headerSerialized);
+                                      canonData.encFields_c, encryptedItems, canonData.data_c, headerSerialized);
     var footerAttribute := footer.makeTerminal();
 
     result := result[HeaderField := headerAttribute];
@@ -633,13 +633,13 @@ module AwsCryptographyDbEncryptionSdkStructuredEncryptionOperations refines Abst
 
     var headerAlgorithmSuite :- head.GetAlgorithmSuite(config.materialProviders);
     var parsedHeader := ParsedHeader(
-        cryptoSchema := canonData.cryptoSchema,
-        algorithmSuiteId := headerAlgorithmSuite.id.DBE,
-        encryptedDataKeys := head.dataKeys,
-        storedEncryptionContext := head.encContext,
-        encryptionContext := mat.encryptionContext
+      cryptoSchema := canonData.cryptoSchema,
+      algorithmSuiteId := headerAlgorithmSuite.id.DBE,
+      encryptedDataKeys := head.dataKeys,
+      storedEncryptionContext := head.encContext,
+      encryptionContext := mat.encryptionContext
     );
-    
+
     var encryptOutput := EncryptStructureOutput(
       encryptedStructure := StructuredData(
         content := StructuredDataContent.DataMap(
@@ -655,21 +655,21 @@ module AwsCryptographyDbEncryptionSdkStructuredEncryptionOperations refines Abst
   predicate DecryptStructureEnsuresPublicly(
     input: DecryptStructureInput,
     output: Result<DecryptStructureOutput, Error>) {
-      // Input and output types must be the same, and this constraint is useful to Dafny users
+    // Input and output types must be the same, and this constraint is useful to Dafny users
     && (output.Success? && input.encryptedStructure.content.DataMap? ==> output.value.plaintextStructure.content.DataMap?)
     && (output.Success? && input.encryptedStructure.content.DataList? ==> output.value.plaintextStructure.content.DataList?)
     && (output.Success? && input.encryptedStructure.content.Terminal? ==> output.value.plaintextStructure.content.Terminal?)
-      // Ensure the CryptoSchema in the ParsedHeader is consistent with the input authenticateSchema
+       // Ensure the CryptoSchema in the ParsedHeader is consistent with the input authenticateSchema
     && (output.Success? ==>
-      // For now we only support decrypting flat maps
-      && output.value.parsedHeader.cryptoSchema.content.SchemaMap?
-      && var cryptoMap := output.value.parsedHeader.cryptoSchema.content.SchemaMap;
-      && CryptoSchemaMapIsFlat(cryptoMap)
-      && input.authenticateSchema.content.SchemaMap?
-      && var authMap := input.authenticateSchema.content.SchemaMap;
-      && AuthSchemaIsFlat(authMap)
-      && ValidString(input.tableName)
-      && ValidParsedCryptoSchema(cryptoMap, authMap + ReservedAuthMap, input.tableName))
+          // For now we only support decrypting flat maps
+          && output.value.parsedHeader.cryptoSchema.content.SchemaMap?
+          && var cryptoMap := output.value.parsedHeader.cryptoSchema.content.SchemaMap;
+          && CryptoSchemaMapIsFlat(cryptoMap)
+          && input.authenticateSchema.content.SchemaMap?
+          && var authMap := input.authenticateSchema.content.SchemaMap;
+          && AuthSchemaIsFlat(authMap)
+          && ValidString(input.tableName)
+          && ValidParsedCryptoSchema(cryptoMap, authMap + ReservedAuthMap, input.tableName))
   }
 
   predicate ValidParsedCryptoSchema(cryptoSchema: CryptoSchemaMap, authSchema: AuthenticateSchemaMap, tableName: GoodString)
@@ -678,16 +678,16 @@ module AwsCryptographyDbEncryptionSdkStructuredEncryptionOperations refines Abst
   {
     // Every field in the crypto map exists in the auth map as SIGN
     && (forall k <- cryptoSchema.Keys :: k in authSchema && authSchema[k].content.Action.SIGN?)
-    // The crypto map is not missing any SIGN fields from the auth map
+       // The crypto map is not missing any SIGN fields from the auth map
     && (forall kv <- authSchema.Items | kv.1.content.Action.SIGN? :: kv.0 in cryptoSchema.Keys)
-    // Every field in the crypto map is ENCRYPT_AND_SIGN, CONTEXT_AND_SIGN or SIGN_ONLY
+       // Every field in the crypto map is ENCRYPT_AND_SIGN, CONTEXT_AND_SIGN or SIGN_ONLY
     && (forall v <- cryptoSchema.Values :: IsAuthAttr(v.content.Action))
   }
 
   const ReservedAuthMap : AuthSchemaPlain := map[
-    HeaderField := DoNotSign, // The header field is authenticated in the footer via a separate mechanism
-    FooterField := DoNotSign
-  ]
+                                               HeaderField := DoNotSign, // The header field is authenticated in the footer via a separate mechanism
+                                               FooterField := DoNotSign
+                                             ]
 
   function method SafeDecode(data : CMP.Utf8Bytes) : string
   {
@@ -733,67 +733,67 @@ module AwsCryptographyDbEncryptionSdkStructuredEncryptionOperations refines Abst
     //# This operation MUST output a [Structured Data](#structured-data) with the following specifics:
     returns (output: Result<DecryptStructureOutput, Error>)
     ensures output.Success? ==>
-      && input.encryptedStructure.content.DataMap?
-      && DataMapIsFlat(input.encryptedStructure.content.DataMap)
-      && var encRecord := input.encryptedStructure.content.DataMap;
+              && input.encryptedStructure.content.DataMap?
+              && DataMapIsFlat(input.encryptedStructure.content.DataMap)
+              && var encRecord := input.encryptedStructure.content.DataMap;
 
-      //= specification/structured-encryption/decrypt-structure.md#parse-the-header
-      //= type=implication
-      //# Given the [input Structured Data](#structured-data),
-      //# this operation MUST access the [Terminal Data](./structures.md#terminal-data)
-      //# at the "aws_dbe_head"
+              //= specification/structured-encryption/decrypt-structure.md#parse-the-header
+              //= type=implication
+              //# Given the [input Structured Data](#structured-data),
+              //# this operation MUST access the [Terminal Data](./structures.md#terminal-data)
+              //# at the "aws_dbe_head"
 
-      //= specification/structured-encryption/decrypt-structure.md#parse-the-header
-      //= type=implication
-      //# The [Terminal Type Id](./structures.md#terminal-type-id) on this Terminal Data MUST be `0xFFFF`.
-      && NeedBinary(encRecord, HeaderField).Pass?
+              //= specification/structured-encryption/decrypt-structure.md#parse-the-header
+              //= type=implication
+              //# The [Terminal Type Id](./structures.md#terminal-type-id) on this Terminal Data MUST be `0xFFFF`.
+              && NeedBinary(encRecord, HeaderField).Pass?
 
-      //= specification/structured-encryption/decrypt-structure.md#verify-signatures
-      //= type=implication
-      //# A footer field MUST exist with the name `aws_dbe_foot`
+              //= specification/structured-encryption/decrypt-structure.md#verify-signatures
+              //= type=implication
+              //# A footer field MUST exist with the name `aws_dbe_foot`
 
-      //= specification/structured-encryption/decrypt-structure.md#verify-signatures
-      //= type=implication
-      //# The footer field TypeID MUST be 0xFFFF
-      && NeedBinary(encRecord, FooterField).Pass?
+              //= specification/structured-encryption/decrypt-structure.md#verify-signatures
+              //= type=implication
+              //# The footer field TypeID MUST be 0xFFFF
+              && NeedBinary(encRecord, FooterField).Pass?
 
-      //= specification/structured-encryption/decrypt-structure.md#authenticate-schema
-      //= type=implication
-      //# The Authenticate Schema MUST explicitly configure a [Authenticate Action](./structures.md#authenticate-action) for every
-      //# [Terminal Data](./structures.md#terminal-data) that exists on the [input Structured Data](#structured-data),
-      //# and MUST NOT describe Authenticate Actions for locations within the input Structured Data that either
-      //# do not exist, or contain non-Terminal Data structures;
-      //# otherwise, this operation operation MUST yield an error.
-      && input.authenticateSchema.content.SchemaMap?
-      && input.authenticateSchema.content.SchemaMap.Keys + ReservedAuthMap.Keys == input.encryptedStructure.content.DataMap.Keys
+              //= specification/structured-encryption/decrypt-structure.md#authenticate-schema
+              //= type=implication
+              //# The Authenticate Schema MUST explicitly configure a [Authenticate Action](./structures.md#authenticate-action) for every
+              //# [Terminal Data](./structures.md#terminal-data) that exists on the [input Structured Data](#structured-data),
+              //# and MUST NOT describe Authenticate Actions for locations within the input Structured Data that either
+              //# do not exist, or contain non-Terminal Data structures;
+              //# otherwise, this operation operation MUST yield an error.
+              && input.authenticateSchema.content.SchemaMap?
+              && input.authenticateSchema.content.SchemaMap.Keys + ReservedAuthMap.Keys == input.encryptedStructure.content.DataMap.Keys
 
-      //= specification/structured-encryption/decrypt-structure.md#authenticate-schema
-      //= type=implication
-      //# The Authenticate Schema MUST include at least one [SIGN Authenticate Action](./structures.md#sign);
-      //# otherwise, this operation MUST yield an error.
-      && AuthSchemaIsFlat(input.authenticateSchema.content.SchemaMap)
-      && (exists x :: (x in input.authenticateSchema.content.SchemaMap && input.authenticateSchema.content.SchemaMap[x].content.Action == SIGN))
+              //= specification/structured-encryption/decrypt-structure.md#authenticate-schema
+              //= type=implication
+              //# The Authenticate Schema MUST include at least one [SIGN Authenticate Action](./structures.md#sign);
+              //# otherwise, this operation MUST yield an error.
+              && AuthSchemaIsFlat(input.authenticateSchema.content.SchemaMap)
+              && (exists x :: (x in input.authenticateSchema.content.SchemaMap && input.authenticateSchema.content.SchemaMap[x].content.Action == SIGN))
 
-      && var headerSerialized := encRecord[HeaderField].content.Terminal.value;
-      //= specification/structured-encryption/decrypt-structure.md#parse-the-header
-      //= type=implication
-      //# This operation MUST deserialize the header bytes
-      //# according to the [header format](./header.md).
-      && Header.PartialDeserialize(headerSerialized).Success?
-      && var head := Header.PartialDeserialize(headerSerialized).value;
+              && var headerSerialized := encRecord[HeaderField].content.Terminal.value;
+              //= specification/structured-encryption/decrypt-structure.md#parse-the-header
+              //= type=implication
+              //# This operation MUST deserialize the header bytes
+              //# according to the [header format](./header.md).
+              && Header.PartialDeserialize(headerSerialized).Success?
+              && var head := Header.PartialDeserialize(headerSerialized).value;
 
-      //= specification/structured-encryption/decrypt-structure.md#construct-decrypted-structured-data
-      //= type=implication
-      //# - [Terminal Data](./structures.md#terminal-data) MUST NOT exist at the "aws_dbe_head"
-      //# or "aws_dbe_foot".
-      && HeaderField !in output.value.plaintextStructure.content.DataMap
-      && FooterField !in output.value.plaintextStructure.content.DataMap
+              //= specification/structured-encryption/decrypt-structure.md#construct-decrypted-structured-data
+              //= type=implication
+              //# - [Terminal Data](./structures.md#terminal-data) MUST NOT exist at the "aws_dbe_head"
+              //# or "aws_dbe_foot".
+              && HeaderField !in output.value.plaintextStructure.content.DataMap
+              && FooterField !in output.value.plaintextStructure.content.DataMap
   {
     :- Need(input.authenticateSchema.content.SchemaMap?, E("Authenticate Schema must be a SchemaMap"));
     :- Need(AuthSchemaIsFlat(input.authenticateSchema.content.SchemaMap), E("Schema must be flat."));
     :- Need(forall k <- input.authenticateSchema.content.SchemaMap :: ValidString(k), E("Schema has bad field name."));
     :- Need(forall k <- input.authenticateSchema.content.SchemaMap | k in ReservedAuthMap ::
-      input.authenticateSchema.content.SchemaMap[k] == ReservedAuthMap[k], E("Reserved fields in Schema must be DO_NOT_SIGN."));
+              input.authenticateSchema.content.SchemaMap[k] == ReservedAuthMap[k], E("Reserved fields in Schema must be DO_NOT_SIGN."));
     var authSchema : AuthSchemaPlain := input.authenticateSchema.content.SchemaMap + ReservedAuthMap;
 
     :- Need(input.encryptedStructure.content.DataMap?, E("Input structure must be a DataMap"));
@@ -885,15 +885,15 @@ module AwsCryptographyDbEncryptionSdkStructuredEncryptionOperations refines Abst
     //= specification/structured-encryption/decrypt-structure.md#verify-signatures
     //# Decryption MUST fail immediately if verification fails.
     var _ :- footer.validate(config.primitives, mat, head.dataKeys,
-                            canonData.signedFields_c, canonData.encFields_c, map[], canonData.data_c, headerSerialized);
+                             canonData.signedFields_c, canonData.encFields_c, map[], canonData.data_c, headerSerialized);
     var decryptedItems :- Crypt.Decrypt(config.primitives, postCMMAlg, key, head, canonData.encFields_c, canonData.data_c);
 
     var result : map<string, StructuredData> := map k <- encRecord | true :: k :=
-      var c := Paths.SimpleCanon(input.tableName, k);
-      if c in decryptedItems then
-        decryptedItems[c]
-      else
-        encRecord[k];
+                                                                          var c := Paths.SimpleCanon(input.tableName, k);
+                                                                          if c in decryptedItems then
+                                                                            decryptedItems[c]
+                                                                          else
+                                                                            encRecord[k];
 
     //= specification/structured-encryption/decrypt-structure.md#construct-decrypted-structured-data
     //# - For every [input Terminal Data](./structures.md#terminal-data) in the [input Structured Data](#structured-data)
@@ -928,11 +928,11 @@ module AwsCryptographyDbEncryptionSdkStructuredEncryptionOperations refines Abst
     //#   - [Stored Encryption Context](./header.md#encryption-context): The Encryption Context stored in the header.
     //#   - [Encrypted Data Keys](./header.md#encrypted-data-keys): The Encrypted Data Keys stored in the header.
     var parsedHeader := ParsedHeader(
-        cryptoSchema := canonData.cryptoSchema,
-        algorithmSuiteId := headerAlgorithmSuite.id.DBE,
-        encryptedDataKeys := head.dataKeys,
-        storedEncryptionContext := head.encContext,
-        encryptionContext := mat.encryptionContext
+      cryptoSchema := canonData.cryptoSchema,
+      algorithmSuiteId := headerAlgorithmSuite.id.DBE,
+      encryptedDataKeys := head.dataKeys,
+      storedEncryptionContext := head.encContext,
+      encryptionContext := mat.encryptionContext
     );
 
     var decryptOutput := DecryptStructureOutput(
